src/educational/functional/TreeSort.dfy
@@ -1,0 +1,48 @@
+include "./BST.dfy"
+
+// ------------------------------------ Function Methods ---------------------------------------- //
+
+/** Properties:
+ *
+ *  Lemma_TreeSortIntegrity
+ *    ==> ensures List_ToMultiset(TreeSort(list)) == List_ToMultiset(list)
+ *
+ *  Lemma_TreeSortOrdering(list)
+ *    ==> ensures list_ordered(TreeSort(list))
+ *
+ */
+function method TreeSort(list:List<int>) : (sortedList:List<int>)
+  decreases list
+{
+  BST_InOrder(BST_Load(list))
+}
+
+// ------------------------------------- TreeSort Lemmas ---------------------------------------- //
+
+lemma Lemma_TreeSortIntegrity(list:List<T>)
+  ensures List_ToMultiset(TreeSort(list)) == List_ToMultiset(list)
+{
+  calc == {
+    List_ToMultiset(TreeSort(list));
+      { assert TreeSort(list) == BST_InOrder(BST_Load(list)); }
+    List_ToMultiset(BST_InOrder(BST_Load(list)));
+      { Lemma_BSTInOrderIntegrity(BST_Load(list)); }
+    BST_ToMultiset(BST_Load(list));
+      { Lemma_BSTLoadIntegrity(list); }
+    List_ToMultiset(list);
+  }
+}
+
+lemma Lemma_TreeSortOrdering(list:List<T>)
+  ensures list_ordered(TreeSort(list))
+{
+  calc == {
+    list_ordered(TreeSort(list));
+      { assert TreeSort(list) == BST_InOrder(BST_Load(list)); }
+    list_ordered(BST_InOrder(BST_Load(list)));
+      { Lemma_BSTLoadOrdering(list); }
+      { assert bst_ordered(BST_Load(list)); }
+      { Lemma_BSTInOrderOrdering(BST_Load(list)); }
+    true;
+  }
+}
