src/production/fibonacci/Fibonacci.dfy
@@ -1,0 +1,106 @@
+
+// ----------------------------------- Fibonacci_Recursive -------------------------------------- //
+
+function method Fibonacci_Recursive(n: nat): nat
+  decreases n
+{
+  if (n == 0) then 0 else
+  if (n == 1) then 1 else
+  Fibonacci_Recursive(n-2) + Fibonacci_Recursive(n-1)
+}
+
+// --------------------------------- Fibonacci_TailRecursive ------------------------------------ //
+
+/** Properties:
+ *
+ *  Lemma_FibonacciTailRecursiveEqualsFibonacciRecursive(n: nat, i: nat)
+ *    ==> Fibonacci_TailRecursive(n-i, Fibonacci_Recursive(i), Fibonacci_Recursive(i+1)) == Fibonacci_Recursive(n)
+ *
+ *  Note: Initial call should be with a=0 and b=1
+ *
+ */
+function method Fibonacci_TailRecursive(n: nat, a: nat, b: nat): nat
+  decreases n
+{
+  if (n == 0) then a else
+  Fibonacci_TailRecursive(n-1, b, a+b)
+}
+
+// --------------------------------- Fibonacci_RecursivePair ------------------------------------ //
+
+/** Properties:
+ *
+ *  Lemma_FibonacciRecursivePairEqualsFibonacciRecursive(n) 
+ *    ==> ensures Fibonacci_RecursivePair(n) == Fibonacci_Recursive(n)
+ *
+ */
+function method Fibonacci_RecursivePair(n: nat): nat
+{
+  match Fibonacci_RecursivePairAux(n) {
+    case (a, b) => a
+  }
+}
+
+/** Properties:
+ *
+ *  Lemma_FibonacciRecursivePairAuxEqualsFibonacciRecursive(n) 
+ *    ==> ensures Fibonacci_RecursivePairAux(n) == (Fibonacci_Recursive(n), Fibonacci_Recursive(n+1))
+ *
+ */
+function method Fibonacci_RecursivePairAux(n: nat): (nat, nat)
+  decreases n
+{
+  if (n == 0) then (0, 1) else
+  match Fibonacci_RecursivePairAux(n-1) {
+    case (a, b) => (b, a+b)
+  }
+}
+
+// ----------------------------------- Fibonacci_Iterative -------------------------------------- //
+
+method Fibonacci_Iterative(n: nat) returns (a: nat)
+  ensures a == Fibonacci_Recursive(n)
+{
+  a := 0;
+  var b: nat := 1;
+  var i: nat := 0;
+
+  while i < n
+    invariant 0 <= i <= n
+    invariant a == Fibonacci_Recursive(i)
+    invariant b == Fibonacci_Recursive(i+1)
+    decreases n-i
+  {
+    a, b := b, a+b;
+    i := i+1;
+  }
+}
+
+// ------------------------------- Fibonacci_TailRecursive Lemmas ------------------------------- //
+
+lemma {:induction n, i} Lemma_FibonacciTailRecursiveEqualsFibonacciRecursive(n: nat, i: nat)
+  requires 0 <= n
+  requires 0 <= i <= n
+  ensures Fibonacci_TailRecursive(n-i, Fibonacci_Recursive(i), Fibonacci_Recursive(i+1)) == Fibonacci_Recursive(n)
+  decreases n-i
+{
+  if (n-i > 0) {
+    calc == {
+      Fibonacci_TailRecursive(n-i, Fibonacci_Recursive(i), Fibonacci_Recursive(i+1));
+      Fibonacci_TailRecursive(n-i-1, Fibonacci_Recursive(i+1), Fibonacci_Recursive(i+2));
+        { Lemma_FibonacciTailRecursiveEqualsFibonacciRecursive(n, i+1); }
+      Fibonacci_Recursive(n);
+    }
+  }
+}
+
+// ------------------------------- Fibonacci_RecursivePair Lemmas ------------------------------- //
+
+lemma {:induction n} Lemma_FibonacciRecursivePairEqualsFibonacciRecursive(n: nat)
+  ensures Fibonacci_RecursivePair(n) == Fibonacci_Recursive(n)
+{ }
+
+lemma {:induction n} Lemma_FibonacciRecursivePairAuxEqualsFibonacciRecursive(n: nat)
+  ensures Fibonacci_RecursivePairAux(n) == (Fibonacci_Recursive(n), Fibonacci_Recursive(n+1))
+  decreases n
+{ }
