src/production/functional/BST.dfy
@@ -1,0 +1,292 @@
+include "./List.dfy"
+
+// --------------------------------------- Datatypes -------------------------------------------- //
+
+datatype Leaf = Nil
+datatype BST<T> = Leaf | Node(left:BST<T>, data:T, right:BST<T>)
+
+// --------------------------------------- Predicates ------------------------------------------- //
+
+predicate bst_ordered(tree:BST<T>)
+  decreases tree
+{
+  match tree {
+    case Leaf => true
+    case Node(left, x, right) =>
+      bst_ordered(left) &&
+      bst_ordered(right) &&
+      bst_upper_bound(left, x) &&
+      bst_lower_bound(right, x)
+  }
+}
+
+predicate bst_lower_bound(tree:BST<T>, d:T)
+  decreases tree
+{
+  match tree {
+    case Leaf => true
+    case Node(left, x, right) => d <= x && bst_lower_bound(left, d) && bst_lower_bound(right, d)
+  }
+}
+
+predicate bst_upper_bound(tree:BST<T>, d:T)
+  decreases tree
+{
+  match tree {
+    case Leaf => true
+    case Node(left, x, right) => d >= x && bst_upper_bound(left, d) && bst_upper_bound(right, d)
+  }
+}
+
+// ------------------------------------ Function Methods ---------------------------------------- //
+
+function method BST_ToMultiset(tree:BST<T>) : multiset<T>
+  decreases tree
+{
+  match tree {
+    case Leaf => multiset{}
+    case Node(left, x, right) => multiset{x} + BST_ToMultiset(left) + BST_ToMultiset(right)
+  }
+}
+
+/** Properties:
+ *
+ *  Lemma_BSTInsertIntegrity(tree, d)
+ *    ==> ensures BST_ToMultiset(tree) + multiset{d} == BST_ToMultiset(BST_Insert(tree, d))
+ *
+ *  Lemma_BSTInsertOrdering(tree, d)
+ *    ==> ensures bst_ordered(BST_Insert(tree, d))
+ *
+ *  Lemma_BSTInsertUpperBound(tree, d, b)
+ *    ==> ensures bst_upper_bound(BST_Insert(tree, d), b)
+ *
+ *  Lemma_BSTInsertLowerBound(tree, d, b)
+ *    ==> ensures bst_lower_bound(BST_Insert(tree, d), b)
+ *
+ */
+function method BST_Insert(tree:BST<T>, d:T) : (result:BST<T>)
+  decreases tree
+{
+  match tree {
+    case Leaf => Node(Leaf, d, Leaf)
+    case Node(left, x, right) =>
+      if (d < x) then
+        Node(BST_Insert(left, d), x , right)
+      else
+        Node(left, x, BST_Insert(right, d))
+  }
+}
+
+/** Properties:
+ *
+ *  Lemma_BSTLoadIntegrity(list:List<T>)
+ *    ==> ensures List_ToMultiset(list) == BST_ToMultiset(BST_Load(list))
+ *
+*  Lemma_BSTLoadOrdering(list)
+ *    ==> ensures bst_ordered(BST_Load(list))
+ *
+ */
+function method BST_Load(list:List<T>) : (tree:BST<T>)
+  decreases list
+{
+  match list {
+    case List_Empty => Leaf
+    case Cons(head, tail) => BST_Insert(BST_Load(tail), head)
+  }
+}
+
+/** Properties:
+ *
+ *  Lemma_BSTInOrderIntegrity(tree)
+ *    ==> ensures List_ToMultiset(BST_InOrder(tree)) == BST_ToMultiset(tree)
+ *
+ *  Lemma_BSTInOrderOrdering(tree)
+ *    ==> ensures list_ordered(BST_InOrder(tree))
+ *
+ *  Lemma_BSTInOrderUpperBound(tree, d)
+ *    ==> ensures list_upper_bound(BST_InOrder(tree), d)
+ *
+ *  Lemma_BSTInOrderLowerBound(tree, d)
+ *    ==> ensures list_lower_bound(BST_InOrder(tree), d)
+ *
+ */
+function method BST_InOrder(tree:BST<T>) : (result:List<T>)
+  decreases tree
+{
+  match tree {
+    case Leaf => List_Empty
+    case Node(left, x, right) => 
+      List_Concat(BST_InOrder(left), Cons(x, BST_InOrder(right)))
+  }
+}
+
+// ------------------------------------ BST_Insert Lemmas --------------------------------------- //
+
+lemma {:induction tree} Lemma_BSTInsertIntegrity(tree:BST<T>, d:T)
+  ensures BST_ToMultiset(BST_Insert(tree, d)) == BST_ToMultiset(tree) + multiset{d}
+  decreases tree
+{ }
+
+lemma {:induction tree} Lemma_BSTInsertOrdering(tree:BST<T>, d:T)
+  requires bst_ordered(tree)
+  ensures bst_ordered(BST_Insert(tree, d))
+  decreases tree
+{
+  match tree {
+    case Leaf =>
+      calc == {
+        bst_ordered(BST_Insert(Leaf, d));
+        bst_ordered(Node(Leaf, d, Leaf));
+        true;
+      }
+    case Node(left, x, right) =>
+      calc == {
+        bst_ordered(BST_Insert(tree, d));
+        bst_ordered(BST_Insert(Node(left, x, right), d));
+        { if (d < x) {
+          calc == {
+            bst_ordered(Node(BST_Insert(left, d), x, right));
+              { Lemma_BSTInsertUpperBound(left, d, x); }
+              { Lemma_BSTInsertOrdering(left, d); }
+            bst_ordered(Node(Leaf, d, Leaf));
+          }
+        } else {
+          calc == {
+            bst_ordered(Node(left, x, BST_Insert(right, d)));
+              { Lemma_BSTInsertLowerBound(right, d, x); }
+              { Lemma_BSTInsertOrdering(right, d); }
+            bst_ordered(Node(Leaf, d, Leaf));
+          }
+        } }
+        true;
+      }
+  }
+}
+
+lemma {:induction tree} Lemma_BSTInsertUpperBound(tree:BST<T>, d:T, b:T)
+  requires bst_ordered(tree)
+  requires bst_upper_bound(tree, b)
+  requires b > d
+  ensures bst_upper_bound(BST_Insert(tree, d), b)
+  decreases tree
+{ }
+
+lemma {:induction tree} Lemma_BSTInsertLowerBound(tree:BST<T>, d:T, b:T)
+  requires bst_ordered(tree)
+  requires bst_lower_bound(tree, b)
+  requires b <= d
+  ensures bst_lower_bound(BST_Insert(tree, d), b)
+  decreases tree
+{ }
+
+// ------------------------------------- BST_Load Lemmas ---------------------------------------- //
+
+lemma {:induction list} Lemma_BSTLoadIntegrity(list:List<T>)
+  ensures BST_ToMultiset(BST_Load(list)) == List_ToMultiset(list)
+  decreases list
+{
+  match list {
+    case List_Empty =>
+    case Cons(head, tail) =>
+      calc == {
+        BST_ToMultiset(BST_Load(Cons(head, tail)));
+        BST_ToMultiset(BST_Insert(BST_Load(tail), head));
+          { Lemma_BSTInsertIntegrity(BST_Load(tail), head); }
+        BST_ToMultiset(BST_Load(tail)) + multiset{head};
+          { Lemma_BSTLoadIntegrity(tail); }
+        List_ToMultiset(list);
+      }
+  }
+}
+
+lemma {:induction list} Lemma_BSTLoadOrdering(list:List<T>)
+  ensures bst_ordered(BST_Load(list))
+  decreases list
+{
+  match list {
+    case List_Empty =>
+    case Cons(head, tail) =>
+      calc == {
+        bst_ordered(BST_Load(Cons(head, tail)));
+        bst_ordered(BST_Insert(BST_Load(tail), head));
+          { Lemma_BSTInsertOrdering(BST_Load(tail), head); }
+        true;
+      }
+  }
+}
+
+// ----------------------------------- BST_InOrder Lemmas --------------------------------------- //
+
+lemma {:induction tree} Lemma_BSTInOrderIntegrity(tree:BST<T>)
+  ensures BST_ToMultiset(tree) == List_ToMultiset(BST_InOrder(tree))
+  decreases tree
+{
+  match tree {
+    case Leaf =>
+    case Node(left, x, right) =>
+      calc == {
+        List_ToMultiset(BST_InOrder(Node(left, x, right)));
+        List_ToMultiset(List_Concat(BST_InOrder(left), Cons(x, BST_InOrder(right))));
+          { Lemma_ListConcatIntegrity(BST_InOrder(left), Cons(x, BST_InOrder(right))); }
+        List_ToMultiset(BST_InOrder(left)) + List_ToMultiset(Cons(x, BST_InOrder(right)));
+        List_ToMultiset(BST_InOrder(left)) + List_ToMultiset(Cons(x, List_Empty)) + List_ToMultiset(BST_InOrder(right));
+        List_ToMultiset(BST_InOrder(left)) + multiset{x} + List_ToMultiset(List_Empty) + List_ToMultiset(BST_InOrder(right));
+        List_ToMultiset(BST_InOrder(left)) + multiset{x} + List_ToMultiset(BST_InOrder(right));
+          { Lemma_BSTInOrderIntegrity(left); }
+          { Lemma_BSTInOrderIntegrity(right); }
+        BST_ToMultiset(tree);
+      }
+  }
+}
+
+lemma {:induction tree} Lemma_BSTInOrderOrdering(tree:BST<T>)
+  requires bst_ordered(tree)
+  ensures list_ordered(BST_InOrder(tree))
+{
+  match tree {
+    case Leaf =>
+    case Node(left, x, right) =>
+      calc == {
+        list_ordered(BST_InOrder(Node(left, x, right)));
+        list_ordered(List_Concat(BST_InOrder(left), Cons(x, BST_InOrder(right))));
+          { Lemma_BSTInOrderLowerBound(right, x); }
+          { Lemma_BSTInOrderUpperBound(left, x); }
+          { Lemma_ListConcatWithMidElemOrdering(BST_InOrder(left), x, BST_InOrder(right)); }
+        true;
+      }
+  }
+}
+
+lemma {:induction tree} Lemma_BSTInOrderUpperBound(tree:BST<T>, d:T)
+  requires bst_ordered(tree)
+  requires bst_upper_bound(tree, d)
+  ensures list_upper_bound(BST_InOrder(tree), d)
+{
+  match tree {
+    case Leaf =>
+    case Node(left, x, right) =>
+      calc == {
+        list_upper_bound(BST_InOrder(Node(left, x, right)), d);
+        list_upper_bound(List_Concat(BST_InOrder(left), Cons(x, BST_InOrder(right))), d);
+          { Lemma_ListConcatUpperBound(BST_InOrder(left), BST_InOrder(right), d, x); }
+        true;
+      }
+  }
+}
+
+lemma {:induction tree} Lemma_BSTInOrderLowerBound(tree:BST<T>, d:T)
+  requires bst_ordered(tree)
+  requires bst_lower_bound(tree, d)
+  ensures list_lower_bound(BST_InOrder(tree), d)
+{
+  match tree {
+    case Leaf =>
+    case Node(left, x, right) =>
+      calc == {
+        list_lower_bound(BST_InOrder(Node(left, x, right)), d);
+        list_lower_bound(List_Concat(BST_InOrder(left), Cons(x, BST_InOrder(right))), d);
+          { Lemma_ListConcatLowerBound(BST_InOrder(left), BST_InOrder(right), d, x); }
+        true;
+      }
+  }
+}
