src/production/functional/List.dfy
@@ -1,0 +1,103 @@
+type T = int
+
+// --------------------------------------- Datatypes -------------------------------------------- //
+
+datatype List_Empty = Nil
+datatype List<T> = List_Empty | Cons(head:T, tail:List<T>)
+
+// --------------------------------------- Predicates ------------------------------------------- //
+
+predicate list_ordered(list:List<T>)
+  decreases list
+{
+  match list {
+    case List_Empty => true
+    case Cons(head, List_Empty) => true
+    case Cons(head, Cons(ht, tail)) => head <= ht && list_ordered(Cons(ht, tail))
+  }
+}
+
+predicate list_lower_bound(list:List<T>, d:T)
+  decreases list
+{
+  match list {
+    case List_Empty => true
+    case Cons(head, tail) => (d <= head) && list_lower_bound(tail, d)
+  }
+}
+
+predicate list_upper_bound(list:List<T>, d:T)
+  decreases list
+{
+  match list {
+    case List_Empty => true
+    case Cons(head, tail) => (d >= head) && list_upper_bound(tail, d)
+  }
+}
+
+// ------------------------------------ Function Methods ---------------------------------------- //
+
+function method List_ToMultiset(list:List<T>) : (m:multiset<T>)
+  decreases list
+{
+  match list {
+    case List_Empty => multiset{}
+    case Cons(head, tail) => multiset{head} + List_ToMultiset(tail)
+  }
+}
+
+/** Properties:
+ *
+ *  Lemma_ListConcatIntegrity(a, b)
+ *    ==> ensures List_ToMultiset(List_Concat(a, b)) == List_ToMultiset(a) + List_ToMultiset(b)
+ *
+ *  Lemma_ListConcatWithMidElemOrdering(a, x, b)
+ *    ==> ensures list_ordered(List_Concat(a, Cons(x, b)))
+ *
+ *  Lemma_ListConcatUpperBound(a, b, d, x)
+ *    ==> ensures list_upper_bound(List_Concat(a, Cons(x, b)), d)
+ *
+ *  Lemma_ListConcatLowerBound(a, b, d, x)
+ *    ==> ensures list_lower_bound(List_Concat(a, Cons(x, b)), d)
+ *
+ */
+function method List_Concat(a:List<T>, b:List<T>) : List<T>
+  decreases a
+{
+  match a {
+    case List_Empty => b
+    case Cons(head, tail) => Cons(head, List_Concat(tail, b))
+  }
+}
+
+// ------------------------------------ List_Concat Lemmas -------------------------------------- //
+
+lemma {:induction a} Lemma_ListConcatIntegrity(a:List<T>, b:List<T>)
+  ensures List_ToMultiset(List_Concat(a, b)) == List_ToMultiset(a) + List_ToMultiset(b)
+  decreases a, b
+{ }
+
+lemma {:induction a, b} Lemma_ListConcatWithMidElemOrdering(a:List<T>, x:T, b:List<T>)
+  requires list_ordered(a)
+  requires list_ordered(b)
+  requires list_lower_bound(b, x)
+  requires list_upper_bound(a, x)
+  ensures list_ordered(List_Concat(a, Cons(x, b)))
+  decreases a, b
+{ }
+
+lemma {:induction listLeft} Lemma_ListConcatUpperBound(listLeft:List<T>, listRight:List<T>, d:T, x:T)
+  requires list_upper_bound(listLeft, d)
+  requires list_upper_bound(listRight, d)
+  requires d >= x
+  ensures list_upper_bound(List_Concat(listLeft, Cons(x, listRight)), d)
+  decreases listLeft
+{ }
+
+lemma {:induction listLeft} Lemma_ListConcatLowerBound(listLeft:List<T>, listRight:List<T>, d:T, x:T)
+  requires list_lower_bound(listLeft, d)
+  requires list_lower_bound(listRight, d)
+  requires d <= x
+  ensures list_lower_bound(List_Concat(listLeft, Cons(x, listRight)), d)
+  decreases listLeft
+{ }
