src/production/functional/TreeSort.dfy
@@ -19,31 +19,23 @@ function method TreeSort(list:List<int>) : (sortedList:List<int>)
 
 // ------------------------------------- TreeSort Lemmas ---------------------------------------- //
 
-lemma {:induction list} Lemma_TreeSortIntegrity(list:List<T>)
+lemma Lemma_TreeSortIntegrity(list:List<T>)
   ensures List_ToMultiset(TreeSort(list)) == List_ToMultiset(list)
 {
   calc == {
     List_ToMultiset(TreeSort(list));
-      { assert TreeSort(list) == BST_InOrder(BST_Load(list)); }
-    List_ToMultiset(BST_InOrder(BST_Load(list)));
-      { Lemma_BSTLoadOrdering(list); }
-      { assert bst_ordered(BST_Load(list)); }
       { Lemma_BSTInOrderIntegrity(BST_Load(list)); }
-    BST_ToMultiset(BST_Load(list));
       { Lemma_BSTLoadIntegrity(list); }
     List_ToMultiset(list);
   }
 }
 
-lemma {:induction list} Lemma_TreeSortOrdering(list:List<T>)
+lemma Lemma_TreeSortOrdering(list:List<T>)
   ensures list_ordered(TreeSort(list))
 {
   calc == {
     list_ordered(TreeSort(list));
-      { assert TreeSort(list) == BST_InOrder(BST_Load(list)); }
-    list_ordered(BST_InOrder(BST_Load(list)));
       { Lemma_BSTLoadOrdering(list); }
-      { assert bst_ordered(BST_Load(list)); }
       { Lemma_BSTInOrderOrdering(BST_Load(list)); }
     true;
   }
